More cleanup in stlc_strong_db_parsubst.fst

examples/metatheory/stlc_strong_db_parsubst.fst
@@ -52,39 +52,42 @@ val is_renaming : s:sub -> Tot (n:int{  (renaming s  ==> n=0) /\
                                       (~(renaming s) ==> n=1)})
 let is_renaming s = (if excluded_middle (renaming s) then 0 else 1)
 
+val sub_inc_above : nat -> var -> Tot exp
+let sub_inc_above n y = if y<n then EVar y else EVar (y+1)
+
 val sub_inc : var -> Tot exp
-let sub_inc y = EVar (y+1)
+let sub_inc = sub_inc_above 0
 
 val renaming_sub_inc : unit -> Lemma (renaming (sub_inc))
 let renaming_sub_inc _ = ()
 
 let is_var (e:exp) : int = if is_EVar e then 0 else 1
 
-val subst : e:exp -> s:sub -> Pure exp (requires True)
+val subst : s:sub -> e:exp -> Pure exp (requires True)
      (ensures (fun e' -> (renaming s /\ is_EVar e) ==> is_EVar e'))
      (decreases %[is_var e; is_renaming s; e])
-let rec subst e s =
+let rec subst s e =
   match e with
   | EVar x -> s x
 
   | ELam t e1 ->
-     let subst_elam : y:var -> Tot (e:exp{renaming s ==> is_EVar e}) = fun y ->
-       if y=0
-       then EVar y
-       else subst (s (y - 1)) sub_inc in
-     ELam t (subst e1 subst_elam)
+     let subst_elam : y:var -> Tot (e:exp{renaming s ==> is_EVar e}) =
+       fun y -> if y=0
+                then EVar y
+                else subst sub_inc (s (y-1))                   (* shift +1 *)
+     in ELam t (subst subst_elam e1)
 
-  | EApp e1 e2 -> EApp (subst e1 s) (subst e2 s)
+  | EApp e1 e2 -> EApp (subst s e1) (subst s e2)
 
 val subst_elam: s:sub -> Tot sub
 let subst_elam s y =
   if y = 0 then EVar y
-  else subst (s (y-1)) sub_inc
+  else subst sub_inc (s (y-1))
 
 val subst_extensional: s1:sub -> s2:sub{FEq s1 s2} -> e:exp ->
                        Lemma (requires True)
-                             (ensures (subst e s1 = subst e s2))
-                             [SMTPat (subst e s1); SMTPat (subst e s2)]
+                             (ensures (subst s1 e = subst s2 e))
+                             [SMTPat (subst s1 e); SMTPat (subst s2 e)]
 let subst_extensional s1 s2 e = ()
 
 (* subst_beta_gen is a generalization of the substitution we do for
@@ -92,15 +95,15 @@ let subst_extensional s1 s2 e = ()
    (useful for the substitution lemma) *)
 val sub_beta_gen : var -> exp -> Tot sub
 let sub_beta_gen x v = fun y -> if y < x then (EVar y)
-                                else if y = x then v
-                                else (EVar (y-1))
+                                else if y = x then v (* substitute *)
+                                else (EVar (y-1))    (* shift -1 *)
 
 val subst_beta_gen : var -> exp -> exp -> Tot exp
-let subst_beta_gen x v e = subst e (sub_beta_gen x v)
+let subst_beta_gen x v = subst (sub_beta_gen x v)
 
-let subst_beta v e = subst_beta_gen 0 v e
+let subst_beta = subst_beta_gen 0
 
-(* Small-step operational semantics;
+(* Small-step operational semantics; strong / full-beta reduction is
    non-deterministic, so necessarily in inductive form *)
 
 type step : exp -> exp -> Type =
@@ -134,7 +137,7 @@ let extend g x t y = if y < x then g y
 type typing : env -> exp -> typ -> Type =
   | TyVar : #g:env ->
             x:var{is_Some (g x)} ->
-              typing g (EVar x) (Some.v (g x))
+            typing g (EVar x) (Some.v (g x))
   | TyLam : #g:env ->
             t:typ ->
             #e1:exp ->
@@ -166,9 +169,18 @@ let rec progress _ _ h =
                       | ExIntro e1' h1' -> ExIntro (EApp e1' e2) (SApp1 e2 h1'))
 
 
-(* Typing extensional (weaker) and context invariance (stronger) lemmas;
-   Context invariance is actually used in a single place within substitution,
-   for in a specific form of weakening when typing variables. *)
+(* Typing extensional (weaker) and context invariance (stronger) lemmas *)
+
+(* Typing extensional follows directly from functional extensionality
+   (it's also a special case of context invariance below) *)
+
+val typing_extensional : #e:exp -> #g:env -> #t:typ ->
+      h:(typing g e t) -> g':env{FEq g g'} ->
+      Tot (typing g' e t)
+let typing_extensional _ _ _ h _ = h
+
+(* Context invariance (actually used in a single place within substitution,
+   for in a specific form of weakening when typing variables) *)
 
 val appears_free_in : x:var -> e:exp -> Tot bool (decreases e)
 let rec appears_free_in x e =
@@ -191,47 +203,18 @@ let rec context_invariance _ _ _ h g' =
   | TyApp h1 h2 ->
     TyApp (context_invariance h1 g') (context_invariance h2 g')
 
-(* This one would follow just by functional extensionality *)
-opaque logic type EnvEqual (g1:env) (g2:env) =
-                 (forall (x:var). g1 x = g2 x)
-
-val typing_extensional : #e:exp -> #g:env -> #t:typ ->
-      h:(typing g e t) -> g':env{EnvEqual g g'} ->
-      Tot (typing g' e t)
-let typing_extensional _ _ _ h g' = context_invariance h g'
-
-(* Lemmas about substitution bellow lambdas and shifting *)
-
-val sub_inc_above : nat -> var -> Tot exp
-let sub_inc_above n y = if y<n then EVar y else EVar (y+1)
+(* Lemmas about substitution and shifting bellow lambdas *)
 
 val shift_up_above : nat -> exp -> Tot exp
-let shift_up_above n e = subst e (sub_inc_above n)
+let shift_up_above n e = subst (sub_inc_above n) e
 
 val shift_up : exp -> Tot exp
 let shift_up = shift_up_above 0
-
-val shift_up_subst_sub_inc : v:exp -> Lemma
-      (ensures (shift_up v = subst v sub_inc))
-let shift_up_subst_sub_inc v =
-  subst_extensional (sub_inc_above 0) sub_inc v
-
-val sub_beta_gen_elam : x:var -> v:exp -> y:var -> Lemma
-      (ensures ((subst_elam (sub_beta_gen  x              v)) y =
-                            (sub_beta_gen (x+1) (shift_up v)) y))
-let sub_beta_gen_elam x v y =
-  if y>0 && x = y-1 then shift_up_subst_sub_inc v
-
-val subst_gen_elam_aux_forall : x:var -> v:exp -> Lemma
-      (ensures (FEq (subst_elam (sub_beta_gen  x  v))
-                    (sub_beta_gen (x+1) (shift_up v))))
-let subst_gen_elam_aux_forall x v = ()
 
 val subst_gen_elam : x:var -> v:exp -> t_y:typ -> e':exp -> Lemma
       (ensures (subst_beta_gen x v (ELam t_y e') =
                 ELam t_y (subst_beta_gen (x+1) (shift_up v) e')))
 let subst_gen_elam x v t_y e' =
-  subst_gen_elam_aux_forall x v;
   subst_extensional (subst_elam (sub_beta_gen  x              v))
                                 (sub_beta_gen (x+1) (shift_up v))  e'
 
@@ -240,7 +223,7 @@ val shift_up_above_lam : n:nat -> t:typ -> e:exp -> Lemma
 let shift_up_above_lam n t e =
   subst_extensional (subst_elam (sub_inc_above n)) (sub_inc_above (n+1)) e
 
-(* Weakening or shifting preserves typing *)
+(* Weakening (or shifting preserves typing) *)
 
 val weakening : x:nat -> #g:env -> #e:exp -> #t:typ -> t':typ ->
       h:typing g e t -> Tot (typing (extend g x t') (shift_up_above x e) t)
@@ -252,8 +235,7 @@ let rec weakening n g v t t' h =
       (shift_up_above_lam n t_y e';
        let h21 = weakening (n+1) t' h21 in
        TyLam t_y (typing_extensional h21 (extend (extend g n t') 0 t_y)))
-  | TyApp h21 h22 -> TyApp (weakening n t' h21)
-                           (weakening n t' h22)
+  | TyApp h21 h22 -> TyApp (weakening n t' h21) (weakening n t' h22)
 
 (* Substitution preserves typing *)
 
@@ -265,7 +247,7 @@ val substitution_preserves_typing :
 let rec substitution_preserves_typing x e v t_x t g h1 h2 =
   match h2 with
   | TyVar y ->
-     if x=y then h1
+     if      x=y then h1
      else if y<x then context_invariance h2 g
      else             TyVar (y-1)
   | TyLam #g' t_y #e' #t' h21 ->
@@ -283,7 +265,7 @@ val preservation : #e:exp -> #e':exp -> hs:step e e' ->
                    #g:env -> #t:typ -> ht:(typing g e t) ->
                    Tot (typing g e' t) (decreases ht)
 let rec preservation e e' hs g t ht =
-  let TyApp #g #e1 #e2 #t11 #t12 h1 h2 = ht in
+  let TyApp h1 h2 = ht in
     match hs with
     | SBeta t e1' e2' -> let TyLam t_x hbody = h1 in
                          substitution_preserves_typing 0 h2 hbody
